Coq/chainmail_properties.v
@@ -1,0 +1,429 @@
+Require Import common.
+Require Import loo_def.
+Require Import loo_properties.
+Require Import loo_reduction_properties.
+Require Import chainmail.
+Require Import function_operations.
+Require Import List.
+Require Import CpdtTactics.
+Require Import Coq.Logic.FunctionalExtensionality.
+
+Lemma adaptation_exists :
+  forall χ1 ϕ1 ψ1
+    χ2 ϕ2 ψ2, finite_ϕ ϕ1 ->
+              finite_ϕ ϕ2 ->
+              not_stuck_ϕ ϕ2 ->
+              forall σ1 σ2, σ1 = (χ1, ϕ1::ψ1) ->
+                       σ2 = (χ2, ϕ2::ψ2) ->
+                       exists σ, σ1 ◁ σ2 ≜ σ.
+Proof.
+  intros; subst.
+
+  inversion H1; subst.
+
+  remember (vMap ϕ1) as β1.
+  remember (vMap ϕ2) as β2.
+  let H := fresh in
+  (destruct (@disjointedness_for_finite_variable_maps value value β1)
+     with (g:=β2)(s:=s)
+    as [f H];
+   try solve [finite_auto; subst; eauto with map_db];
+   destruct H as [f'];
+   andDestruct).
+
+  exists (χ2, (frm (f ∘ β2 ∪ β1) (c_stmt (❲ f' ↦ s ❳))::ψ2)).
+  apply a_adapt
+    with
+      (χ:=χ1)(ψ:=ψ1)(ϕ:=ϕ1)(ϕ':=ϕ2)(c:=contn ϕ1)
+      (β:=β1)(β':=β2)(f':=f')
+      (s:=s)
+      (f:=f);
+    auto with map_db.
+  - destruct ϕ1; crush.
+  - destruct ϕ2; crush.
+Qed.
+
+Hint Resolve adaptation_exists : loo_db.
+
+Lemma adaptation_exists_wf :
+  forall σ1 σ2, σ_wf σ1 ->
+                σ_wf σ2 ->
+                exists σ, σ1 ◁ σ2 ≜ σ.
+Proof.
+  intros σ1 σ2; intros.
+  repeat match goal with
+         | [H : σ_wf ?σ |- _] =>
+           inversion H; subst;
+             clear H
+         end.
+  destruct σ1 as [χ1 ψ1];
+    destruct σ2 as [χ2 ψ2].
+  not_stuck_auto;
+    repeat destruct_exists_loo;
+    simpl in *;
+    andDestruct;
+    subst.
+  unfold finite_σ in *;
+    unfold snd in *.
+  unfold finite_ψ in *.
+  repeat match goal with
+         | [H : forall ϕ', In ϕ' (?ϕ::?ψ) -> finite_ϕ ϕ' |- _ ] =>
+           specialize (H ϕ (in_eq ϕ ψ))
+         end.
+  eauto with loo_db.
+Qed.
+
+
+
+Lemma initial_wf :
+  forall σ, initial σ ->
+       σ_wf σ.
+Proof.
+  intros σ Hinit;
+    inversion Hinit.
+  destruct H as [ϕ];
+    andDestruct;
+    subst.
+  apply config_wf;
+    auto.
+  
+  apply self_config;
+    intros.
+  inversion H;
+    [subst|crush].
+  apply self_frm.
+  exists x, ObjectInstance;
+    split;
+    auto.
+  unfold update, t_update;
+    rewrite eqb_refl;
+    auto.
+  
+  waiting_auto.
+  exists ϕ, nil;
+    simpl;
+    split;
+    intros;
+    crush.
+Qed.
+
+Hint Resolve initial_wf : loo_db.
+
+Lemma fresh_x_ϕ_implies_σ :
+  forall x ϕ A, fresh_x x ϕ A ->
+           forall χ ψ, fresh_x_σ x (χ, ϕ::ψ) A.
+Proof.
+  intros x ϕ A Hfresh χ ψ;
+    unfold fresh_x_σ;
+    exists χ, ϕ, ψ;
+    split;
+    auto.
+Qed.
+
+Hint Resolve fresh_x_ϕ_implies_σ : loo_db.
+
+Lemma fresh_x_σ_implies_ϕ :
+  forall x χ ϕ ψ A, fresh_x_σ x (χ, ϕ::ψ) A ->
+               fresh_x x ϕ A.
+Proof.
+  intros x χ ϕ ψ A Hfresh;
+    unfold fresh_x_σ in *;
+    repeat destruct_exists;
+    andDestruct;
+    match goal with
+    | [H : (_, _) = (_, _) |- _] =>
+      inversion H; subst; clear H
+    end;
+    auto.
+Qed.
+
+Hint Resolve fresh_x_σ_implies_ϕ : loo_db.
+  
+Lemma has_self_update_ϕ_map :
+  forall χ ϕ, has_self_ϕ χ ϕ ->
+         forall x v A, fresh_x x ϕ A ->
+                  has_self_ϕ χ (update_ϕ_map ϕ x v).
+Proof.
+  intros.
+
+  inversion H;
+    subst.
+  apply self_frm.
+  destruct H1 as [α Htmp];
+    destruct Htmp as [o];
+    andDestruct.
+  exists α, o;
+    split;
+    auto.
+  unfold update_ϕ_map, update, t_update;
+    simpl.
+  destruct x as [n];
+    destruct n as [|n'];
+    auto.
+  inversion H0;
+    subst;
+    simpl in *.
+  unfold mapp, stackMap, mapp in H1;
+    unfold this in Ha; rewrite Ha in H1;
+      crush.
+Qed.
+
+Hint Resolve has_self_update_ϕ_map : loo_db.
+
+Lemma has_self_update_ϕ_map_σ :
+  forall χ ϕ, has_self_ϕ χ ϕ ->
+         forall x v ψ A, fresh_x_σ x (χ, ϕ::ψ) A ->
+                    has_self_ϕ χ (update_ϕ_map ϕ x v).
+Proof.
+  intros.
+
+  match goal with
+  | [H : fresh_x_σ _ _ _ |- _] =>
+    inversion H; subst; repeat destruct_exists; andDestruct
+  end.
+  match goal with
+  | [H : (_, _) = (_, _) |- _] => inversion H; subst; clear H
+  end.
+  eauto with loo_db.
+
+Qed.
+
+Hint Resolve has_self_update_ϕ_map_σ : loo_db.
+
+Lemma has_self_update_σ_map :
+  forall σ, has_self_σ σ ->
+       forall x v A, fresh_x_σ x σ A ->
+                has_self_σ (update_σ_map σ x v).
+Proof.
+  intros σ;
+    intros.
+  inversion H0; subst;
+    repeat destruct_exists;
+    andDestruct;
+    subst.
+  auto.
+
+  apply self_config; intros;
+    simpl in *.
+
+  destruct H1; subst.
+
+  - apply has_self_update_ϕ_map with (A:=A); auto.
+    inversion H; subst.
+    apply H2, in_eq.
+
+  - inversion H; subst.
+    apply H3, in_cons; auto.
+Qed.
+
+Hint Resolve has_self_update_σ_map : loo_db.
+
+Lemma wf_update_σ_map :
+  forall σ, σ_wf σ ->
+       forall x α A, fresh_x_σ x σ A ->
+                σ_wf (update_σ_map σ x α).
+Proof.
+  intros σ Hwf; intros.
+  inversion Hwf;
+    subst.
+  apply config_wf;
+    eauto with loo_db.
+Qed.
+
+Lemma adaptation_preserves_mapping :
+  forall σ1 σ2 σ, σ1 ◁ σ2 ≜ σ ->
+             forall z (v : value), mapp σ1 z = Some v ->
+                              mapp σ z = Some v.
+Proof.
+  intros.
+  inversion H;
+    subst.
+
+  repeat map_rewrite; simpl.
+  apply extend_some_2; auto.
+  apply disjoint_dom_symmetry.
+  eapply disjoint_composition; auto with map_db.
+Qed.
+
+Lemma update_fresh_preserves_map :
+  forall x σ A, fresh_x_σ x σ A ->
+           forall z v v', mapp σ z = Some v ->
+                     mapp (update_σ_map σ x v') z = Some v.
+Proof.
+  intros x σ A Hfrsh;
+    inversion Hfrsh;
+    subst;
+    intros.
+
+  unfold fresh_x_σ in *;
+    repeat destruct_exists;
+    andDestruct;
+    subst.
+  match goal with
+  | [H : (_, _) = (_, _) |- _] =>
+    inversion H; subst
+  end.
+  repeat map_rewrite;
+    simpl in *;
+    repeat map_rewrite.
+  inversion Hb; subst.
+  destruct (eq_dec x z);
+    subst;
+    eq_auto;
+    crush.
+Qed.
+
+Lemma fresh_and_elim :
+  forall x σ A1 A2,
+    fresh_x x σ (A1 ∧ A2) ->
+    fresh_x x σ A1 /\ fresh_x x σ A2.
+Proof.
+  intros.
+  inversion H;
+    subst.
+
+  inversion H1;
+    subst;
+    auto with chainmail_db.
+Qed.
+
+Lemma fresh_and_intro :
+  forall x σ A1 A2,
+    fresh_x x σ A1 /\ fresh_x x σ A2 ->
+    fresh_x x σ (A1 ∧ A2).
+Proof.
+  intros.
+  andDestruct.
+  inversion Ha; inversion Hb; subst.
+  apply frsh; auto with chainmail_db.
+Qed.
+
+Lemma fresh_arr_elim :
+  forall x σ A1 A2,
+    fresh_x x σ (A1 ⇒ A2) ->
+    fresh_x x σ A1 /\ fresh_x x σ A2.
+Proof.
+  intros.
+  inversion H;
+    subst.
+
+  inversion H1;
+    subst;
+    auto with chainmail_db.
+Qed.
+
+Lemma fresh_arr_intro :
+  forall x σ A1 A2,
+    fresh_x x σ A1 /\ fresh_x x σ A2 ->
+    fresh_x x σ (A1 ⇒ A2).
+Proof.
+  intros.
+  andDestruct.
+  inversion Ha; inversion Hb; subst.
+  apply frsh; auto with chainmail_db.
+Qed.
+
+Lemma fresh_all_elim :
+  forall x σ A,
+    fresh_x x σ (∀x∙A) ->
+    fresh_x x σ A.
+Proof.
+  intros.
+  inversion H;
+    subst;
+    inversion H1;
+    auto with chainmail_db.
+Qed.
+
+Lemma fresh_all_intro :
+  forall x σ A,
+    fresh_x x σ A ->
+    fresh_x x σ (∀x∙A).
+Proof.
+  intros.
+  inversion H; subst; auto with chainmail_db.
+Qed.
+
+Lemma fresh_notin :
+  forall x σ A1 A2,
+    fresh_x x σ A1 ->
+    notin_Ax A2 x ->
+    fresh_x x σ A2.
+Proof.
+  intros x σ A1 A2 Hfrsh Hnotin.
+  inversion Hfrsh; auto with chainmail_db.
+Qed.
+
+Parameter fresh_exists_for_expression :
+  forall e, exists x, notin_exp e x.
+
+Parameter fresh_exists_for_assertion :
+  forall A, exists x, notin_Ax A x.
+
+
+Parameter fresh_x_exists_for_finite_config :
+  forall σ, finite_σ σ ->
+       forall A, exists x, fresh_x_σ x σ A.
+
+Parameter fresh_address_rename_equality_heap :
+  forall α1 α2 (χ : heap),  χ α1 = None ->
+                       χ α2 = None ->
+                       forall o, update α1 o χ = update α2 o χ.
+
+Parameter fresh_address_rename_equality_state :
+  forall α1 α2 (χ : heap),  χ α1 = None ->
+                       χ α2 = None ->
+                       forall m (x:var), update x (v_addr α1) m = update x (v_addr α2) m.
+
+Lemma initial_heap_wf :
+  forall σ, initial σ ->
+       forall M, M_wf M ->
+            χ_wf M (fst σ).
+Proof.
+  intros σ Hinit;
+    destruct Hinit as [α Hinit];
+    destruct Hinit as [ϕ Hinit];
+    andDestruct;
+    subst;
+    intros.
+  apply heap_wf;
+    intros.
+  simpl in H0; inversion H0; subst.
+  update_auto;
+    [exists ObjectDefn;
+     split; simpl; auto;
+     try solve [obj_defn_rewrite; auto];
+     crush
+    |empty_auto].
+Qed.
+
+Ltac initial_heap_wf_auto :=
+  match goal with
+  | [H : initial ?σ |- χ_wf ?M (fst ?σ)] => eapply initial_heap_wf; eauto
+  end.
+
+Lemma arising_heap_wf :
+  forall M1 M2 σ, arising M1 M2 σ ->
+             M_wf M1 ->
+             M_wf M2 ->
+             forall M, M1 ⋄ M2 ≜ M ->
+                  χ_wf M (fst σ).
+Proof.
+  intros.
+  inversion H; subst.
+  pair_reduces_heap_wf_auto.
+  initial_heap_wf_auto.
+  linking_wf.
+Qed.
+
+Lemma arising_wf :
+  forall M1 M2 σ, arising M1 M2 σ ->
+             σ_wf σ.
+Proof.
+  intros M1 M2 σ Harise.
+  inversion Harise;
+    subst.
+  eapply pair_reductions_preserves_config_wf; eauto with loo_db.
+Qed.
+
+Hint Resolve arising_wf : loo_db.
